Prelims before semantics change

theories/tree_borrows/trees_equal.v
@@ -2201,6 +2201,132 @@ Qed.
       destruct pp; try done. all: repeat (simpl in *; simplify_eq); by econstructor 1.
   Qed.
 
+  (* We can also do symmetric writes, provided we have sufficiently strong preconditions,
+     which include being protected. *)
+  Definition tree_equal_asymmetric_write_pre_protected tr range it acc_tg := 
+    (∀ off, range'_contains range off → 
+            let pp_acc := item_lookup it off in
+            pp_acc.(initialized) = PermInit ∧ pp_acc.(perm) = Active ∧
+            ∀ tg' it', tree_lookup tr tg' it' → 
+            let pp := item_lookup it' off in
+            let rd := rel_dec tr tg' acc_tg in (* flipped here so that it's correcty lined up with logical_state *)
+            match rd with
+            | Child (Strict Immediate) => pp.(perm) = Disabled
+            | Child _ => True
+            | Foreign (Parent _) => pp.(initialized) = PermInit ∧ pp.(perm) = Active (* this follows from state_wf *)
+            | Foreign Cousin => match pp.(perm) with Disabled => True | Reserved InteriorMut _ => ¬ protector_is_active it'.(iprot) C | _ => False end end).
+
+  Lemma tree_equal_asymmetric_write_protected
+    {tr tr' acc_tg range it}
+    (GloballyUnique : forall tg, tree_contains tg tr -> tree_unique tg tr)
+    :
+    (* Accessed tag must be in the tree and protected*)
+    tree_lookup tr acc_tg it ->
+    protector_is_active it.(iprot) C ->
+    tree_equal_asymmetric_write_pre_protected tr range it acc_tg ->
+    (* Under the above conditions if we do a spurious read and it succeeds
+       we get a [tree_equal] on the outcome. *)
+    memory_access AccessWrite C acc_tg range tr = Some tr' ->
+    tree_equal tr tr'.
+  Proof.
+    intros Lkup Protected TreeShapeProper Acc.
+    split; last split.
+    { intro tg. eapply access_preserves_tags. eassumption. }
+    { intros tg1 tg2. eapply access_same_rel_dec. eassumption. }
+    (* That was the easy part, helped by the fact that our initial configuration
+       is reflexivity instead of a more general instance of [tree_equal].
+       Soon it will get more interesting. *)
+    intros tg0 Ex.
+    destruct (unique_implies_lookup (GloballyUnique _ Ex)) as [it0 Lookup0].
+    exists it0.
+    assert (tree_unique tg0 tr') as Unq0'. {
+      erewrite <- tree_apply_access_preserve_unique; last eassumption.
+      apply GloballyUnique. assumption.
+    }
+    destruct (apply_access_spec_per_node (proj1 Lookup0) (proj2 Lookup0) Acc) as
+        (it0' & it0'Spec & Ex0' & Det0').
+    symmetry in it0'Spec.
+    exists it0'.
+    split; first assumption.
+    split; first (split; assumption).
+    (* Now down to per-item reasoning *)
+    intro loc.
+    split; first (eapply item_apply_access_preserves_metadata; eassumption).
+    rewrite bind_Some in it0'Spec; destruct it0'Spec as (perms' & perms'Spec & [= <-]).
+    pose proof (mem_apply_range'_spec _ _ loc _ _ perms'Spec) as PerLoc.
+    clear perms'Spec.
+    assert (itag it0 = tg0) by (eapply tree_determined_specifies_tag; eapply Lookup0).
+    assert (itag it = acc_tg) by (eapply tree_determined_specifies_tag; eapply Lkup).
+    subst.
+    (* Finally the reasoning is per-location *)
+    destruct (decide _) as [HinRange|?]; last first.
+    { rewrite /item_lookup /= PerLoc.
+      constructor. }
+    destruct (TreeShapeProper _ HinRange) as (Htginit&Htgactive&Hothers).
+    (* Keep digging until [apply_access_perm_inner] *)
+    destruct PerLoc as (perm' & perm'Lookup & perm'Spec).
+    pose proof Hothers as Hothers_pure.
+    ospecialize (Hothers _ _ Lookup0).
+    change (default _ _) with (item_lookup it0 loc) in perm'Spec.
+    rewrite {2}/item_lookup perm'Lookup /=.
+    rewrite bind_Some in perm'Spec; destruct perm'Spec as (tmperm & Inner & perm'Spec).
+    rewrite bind_Some in perm'Spec; destruct perm'Spec as (validated & MoreInit & EqPerm).
+    injection EqPerm; clear EqPerm; intros; subst.
+    rewrite rel_dec_flip2 /= in Hothers.
+    destruct (rel_dec tr (itag it) (itag it0)) as [[]|[]] eqn:Hreldec; simpl in Hothers.
+    - assert (∃ tg, tree_contains tg tr ∧ rel_dec tr tg (itag it) = Child (Strict Immediate) ∧ ParentChildIn tg (itag it0) tr) as (tgsw & Hin & Hswdec&Hpar).
+      { rewrite /rel_dec in Hreldec. destruct decide as [HP|HnP]; try done. destruct decide as [HP|?]; try done.
+        destruct HP as [Heq|HSP]. 1: exfalso; eapply HnP; by left.
+        eapply immediate_sandwich in HSP as HSP2. 2, 3: eapply GloballyUnique. 2: eapply Lkup.
+        destruct HSP2 as (tsw&Htsw&HPC). exists tsw.
+        assert (tree_contains tsw tr) as Hcont.
+        { eapply contains_child. 1: right; by eapply Immediate_is_StrictParentChild.
+          eapply Lkup. }
+         split_and!. 1: done. 2: done.
+        rewrite /rel_dec decide_True. 
+        2: right; by eapply Immediate_is_StrictParentChild.
+        rewrite decide_False. 1: by rewrite decide_True.
+        intros HH. eapply immediate_parent_not_child. 4: exact HH. 3: done.
+        all: eapply GloballyUnique. 1: eapply Lkup. done. }
+      assert (∃ itsw, tree_lookup tr tgsw itsw) as (itsw&Hitsw).
+      1: eapply unique_implies_lookup, GloballyUnique, Hin.
+      specialize (Hothers_pure _ _ Hitsw).
+      destruct (apply_access_spec_per_node (proj1 Hitsw) (proj2 Hitsw) Acc) as
+      (itsw' & itsw'Spec & Hitsw'). rewrite Hswdec /= in Hothers_pure.
+      eapply (perm_eq_up_to_C_disabled_parent _ _ _ _ _ tgsw). 3: rewrite /= most_init_comm //=.
+      * econstructor. 2: done. 1: rewrite /rel_dec decide_True //. eapply Hothers_pure.
+      * econstructor. 1: erewrite <- access_same_rel_dec. 2: eassumption. 1: rewrite /rel_dec decide_True //.
+        1: exact Hitsw'. symmetry in itsw'Spec.
+        eapply bind_Some in itsw'Spec as (psw&Hsw&[= Hitsweq]).
+        pose proof (mem_apply_range'_spec _ _ loc _ _ Hsw) as PerLocSW.
+        rewrite decide_True // in PerLocSW. destruct PerLocSW as (p & HPP & Hacc).
+        rewrite /= /apply_access_perm /apply_access_perm_inner /= in Hacc.
+        change (default _ _) with (item_lookup itsw loc) in Hacc.
+        assert (itag itsw = tgsw) as <- by by eapply tree_lookup_correct_tag.
+        rewrite rel_dec_flip2 Hswdec /= Hothers_pure /= in Hacc.
+        rewrite /item_lookup /= -Hitsweq HPP /=.
+        repeat (case_match; simpl in *; try done; simplify_eq).
+    - rewrite /= most_init_comm /=.
+      rewrite /apply_access_perm_inner /= in Inner.
+      destruct (item_lookup it0 loc) as [[] [[] []| | |]] eqn:Hperm, (bool_decide (protector_is_active (iprot it0) C)) eqn:Hprot; simpl in *.
+      all: try by (simplify_eq; first [done | econstructor 1]).
+      all: by eapply bool_decide_eq_true_1 in Hprot.
+    - destruct Hothers as (Hini&Hact).
+      rewrite /apply_access_perm_inner /= in Inner.
+      destruct (item_lookup it0 loc) as [ini pp] eqn:Hperm.
+      simpl in Hini, Hact. subst ini pp. simpl in Inner. simplify_eq. simpl in MoreInit.
+      destruct (bool_decide (protector_is_active (iprot it0) C)); simpl in MoreInit|-*; simplify_eq.
+      all: econstructor 1.
+    - simpl in *. assert (itag it = itag it0) as Htageq.
+      { rewrite /rel_dec in Hreldec. do 2 (destruct decide; try done).
+        eapply mutual_parent_child_implies_equal. 1: done. 1: eapply Lkup. all: done. }
+      assert (it = it0) as ->.
+      { eapply tree_determined_unify. 1, 2: eapply Lkup. rewrite Htageq. eapply Lookup0. }
+      rewrite Htginit in MoreInit|-*. rewrite Htgactive in Inner. simplify_eq.
+      rewrite bool_decide_true // /= in MoreInit. simplify_eq.
+      destruct (item_lookup it0 loc) as [ii pp]. simpl in *; subst ii pp. econstructor 1.
+  Qed.
+
   Lemma apply_within_trees_lift trs fn blk trs' :
     wf_trees trs →
     apply_within_trees fn blk trs = Some trs' →
